conn/props.v
@@ -51,42 +51,30 @@ Context `{!cryptisGS Σ, !heapGS Σ, !connGS Σ}.
 Notation iProp := (iProp Σ).
 
 Implicit Types (cs : state).
-Implicit Types (kI kR kS t : term) (ts : list term).
+Implicit Types (kS t : term) (ts : list term).
+Implicit Types (skI skR : sign_key).
 Implicit Types n m : nat.
 Implicit Types b : bool.
 Implicit Types v : val.
 Implicit Types (ok : Prop) (failed : bool).
 Implicit Types si : sess_info.
 
-Definition failure kI kR : iProp :=
-  compromised_key kI ∨ compromised_key kR.
+Definition failure skI skR : iProp :=
+   public skI ∨ public skR.
 
 Definition wf_sess_info rl si : iProp :=
   minted (si_key si) ∗
-  senc_key (si_key si) ∗
   session rl si.
 
 #[global]
 Instance wf_sess_info_persistent rl si : Persistent (wf_sess_info rl si).
 Proof. apply _. Qed.
 
-Definition never_connected kI kR : iProp :=
-  term_token kR (↑connN.@"server".@kI).
+Definition never_connected skI skR : iProp :=
+  term_token skR (↑connN.@"server".@skI).
 
-Lemma never_connected_switch kI kR Q : ⊢ switch (never_connected kI kR) Q.
+Lemma never_connected_switch skI skR Q : ⊢ switch (never_connected skI skR) Q.
 Proof. apply term_token_switch. Qed.
-
-Lemma public_sencE N rl si t φ :
-  public (TSeal (TKey Seal (si_key si)) (Spec.tag (Tag N) t)) -∗
-  seal_pred N φ -∗
-  wf_sess_info rl si -∗
-  ▷ □ (public (si_key si) ∗ public t ∨ φ (si_key si) t).
-Proof.
-iIntros "#p_m #Nφ #(_ & s_key & sess)".
-iDestruct (public_TSealE with "[//] [//]") as "{p_m} [[p_key p_m]|p_m]".
-- iPoseProof ("s_key" with "p_key") as "{p_key} >p_key". by eauto.
-- iDestruct "p_m" as "[#p_m _]". by eauto.
-Qed.
 
 Definition received_auth si rl n : iProp :=
   term_own (si_share_of rl si) (connN.@"received") (● MaxNat n).
@@ -133,56 +121,54 @@ iInv nroot as "[HP|>recv']".
   case: valid => /= ? _; lia.
 Qed.
 
-Definition connected kI kR rl cs : iProp :=
-  ⌜si_init cs = kI⌝ ∗
-  ⌜si_resp cs = kR⌝ ∗
+Definition connected skI skR rl cs : iProp :=
+  ⌜si_init cs = skI⌝ ∗
+  ⌜si_resp cs = skR⌝ ∗
   ⌜cs_role cs = rl⌝ ∗
   channel (cs_chan cs) ∗
   wf_sess_info (cs_role cs) cs ∗
   ∃ n m, cs_ts cs ↦∗ [ #n; #m ] ∗ received_auth cs (cs_role cs) m.
 
-Lemma connected_channel kI kR rl cs :
-  connected kI kR rl cs -∗
+Lemma connected_channel skI skR rl cs :
+  connected skI skR rl cs -∗
   channel (cs_chan cs).
 Proof. by iIntros "(_ & _ & _ & ? & _)". Qed.
 
-Lemma connected_public_key kI kR rl cs kt :
-  connected kI kR rl cs -∗
+Lemma connected_public_key skI skR rl cs :
+  connected skI skR rl cs -∗
   release_token (si_share_of rl cs) -∗
-  public (TKey kt (si_key cs)) -∗
+  public (si_key cs) -∗
   ◇ compromised_session rl cs.
 Proof.
 iIntros "conn rel #p_k".
 iPoseProof "conn" as "(_ & _ & <- & _ & #sess & _)".
-iDestruct "sess" as "(#? & #s_key & #sess)".
-iPoseProof (senc_key_compromised_keyI with "s_key p_k") as "{p_k} p_k".
-iPoseProof (senc_key_compromised_keyE with "s_key p_k") as "{p_k} >p_k".
-by iApply session_compromised.
+iDestruct "sess" as "(#? & #sess)".
+by iApply (session_compromised with "[] [//] rel").
 Qed.
 
-Lemma connected_released_session kI kR rl cs :
-  connected kI kR rl cs -∗
+Lemma connected_released_session skI skR rl cs :
+  connected skI skR rl cs -∗
   □ (▷ released_session cs → public (si_key cs)).
 Proof.
 iIntros "(_ & _ & _ & _ & #sess & _)".
-by iDestruct "sess" as "(_ & _ & ? & sess)".
+by iDestruct "sess" as "(_ & ? & sess)".
 Qed.
 
-Lemma connected_keyE kI kR rl cs :
-  connected kI kR rl cs -∗
-  ⌜kI = si_init cs⌝ ∗ ⌜kR = si_resp cs⌝ ∗ ⌜rl = cs_role cs⌝.
+Lemma connected_keyE skI skR rl cs :
+  connected skI skR rl cs -∗
+  ⌜skI = si_init cs⌝ ∗ ⌜skR = si_resp cs⌝ ∗ ⌜rl = cs_role cs⌝.
 Proof. by iIntros "(-> & -> & -> & _)". Qed.
 
-Lemma connected_ok kI kR rl cs :
-  connected kI kR rl cs -∗
-  secret kI -∗
-  secret kR -∗
-  sign_key kI -∗
-  sign_key kR -∗
+Lemma connected_ok skI skR rl cs :
+  connected skI skR rl cs -∗
+  secret skI -∗
+  secret skR -∗
+  minted skI -∗
+  minted skR -∗
   ◇ □ ¬ compromised_session rl cs.
 Proof.
 iIntros "(<- & <- & <- & _ & #sess & % & % & _ & _) s_kI s_kR #signI #signR".
-iDestruct "sess" as "(m_k & s_k & sess)".
+iDestruct "sess" as "(m_k & sess)".
 by iApply (session_not_compromised with "[//] s_kI s_kR").
 Qed.
 
